Added cons.v

Cons.v
@@ -58,9 +58,11 @@ Section PerProc.
     then tail (qs idx')
     else qs idx'.
 
+  Definition Hist := list HistElem.
+
   Inductive Spec:
-    HistElem -> State -> Pc -> (Addr -> list Rq) -> list Rp -> bool -> Rob -> Ppc ->
-    HistElem -> State -> Pc -> (Addr -> list Rq) -> list Rp -> bool -> Rob -> Ppc ->
+    Hist -> State -> Pc -> (Addr -> list Rq) -> list Rp -> bool -> Rob -> Ppc ->
+    Hist -> State -> Pc -> (Addr -> list Rq) -> list Rp -> bool -> Rob -> Ppc ->
     TransType -> Prop :=
   | SpecFetch:
       forall h st pc p2m m2p w rob ppc,
@@ -95,7 +97,7 @@ Section PerProc.
         commit rob = Some (pc, Nmh nextPc delS) ->
         getHElem pc st = (nextPc, Nm delS) ->
         Spec h st pc p2m m2p false rob ppc
-             (Nmh pc delS) (updSt st delS) nextPc p2m m2p false rob ppc
+             (Nmh pc delS :: h) (updSt st delS) nextPc p2m m2p false rob ppc
              Internal
   | SpecComStRq:
       forall h st pc p2m m2p rob ppc nextPc a v,
@@ -110,7 +112,7 @@ Section PerProc.
         getHElem pc st = (nextPc, Store a v) ->
         m2p = StoreRp :: xs ->
         Spec h st pc p2m m2p false rob ppc
-             (Storeh pc a v) st nextPc p2m xs false rob ppc
+             (Storeh pc a v :: h) st nextPc p2m xs false rob ppc
              Internal
   | SpecComLoadRq:
       forall h st pc p2m m2p rob ppc nextPc a v delS,
@@ -126,7 +128,7 @@ Section PerProc.
         m2p = LoadCommitRp v :: xs ->
         getLoadDelta pc st v = delS ->
         Spec h st pc p2m m2p false rob ppc
-             (Loadh pc a v delS) (updSt st delS) nextPc p2m xs false rob ppc
+             (Loadh pc a v delS :: h) (updSt st delS) nextPc p2m xs false rob ppc
              Internal
   | SpecComLoadRpBad:
       forall h st pc p2m m2p rob ppc nextPc a v delS xs v' delS',
@@ -136,7 +138,7 @@ Section PerProc.
         v <> v' ->
         getLoadDelta pc st v' = delS' ->
         Spec h st pc p2m m2p false rob ppc
-             (Loadh pc a v' delS') (updSt st delS') nextPc p2m xs false
+             (Loadh pc a v' delS' :: h) (updSt st delS') nextPc p2m xs false
              (empty rob) (set ppc nextPc)
              Internal
   | SpecMemDeqs:
@@ -158,43 +160,39 @@ Section PerProc.
     else mem a'.
 
   Record ProcState :=
-    { hist: HistElem;
+    { hist: Hist;
       getPc: Pc;
       state: State
     }.
 
   Inductive CorrectSystem: (Proc -> ProcState) -> Mem ->
-                           (Proc -> ProcState) -> Mem -> Set :=
+                             (Proc -> ProcState) -> Mem -> Set :=
   | Lod:
       forall p st m a nextPc delS,
         getHElem (getPc (st p)) (state (st p)) = (nextPc, Load a) ->
         getLoadDelta (getPc (st p)) (state (st p)) (m a) = delS ->
         CorrectSystem
           st m
-          (updP st p (Build_ProcState (Loadh (getPc (st p)) a (m a) delS)
+          (updP st p (Build_ProcState (Loadh (getPc (st p)) a (m a) delS :: (hist (st p)))
                                       nextPc (updSt (state (st p)) delS))) m
   | Str:
       forall p st m a nextPc v,
         getHElem (getPc (st p)) (state (st p)) = (nextPc, Store a v) ->
         CorrectSystem
           st m
-          (updP st p (Build_ProcState (Storeh (getPc (st p)) a v)
+          (updP st p (Build_ProcState (Storeh (getPc (st p)) a v :: (hist (st p)))
                                       nextPc (state (st p)))) (updM m a v)
   | NonMem:
       forall p st m nextPc delS,
         getHElem (getPc (st p)) (state (st p)) = (nextPc, Nm delS) ->
         CorrectSystem
           st m
-          (updP st p (Build_ProcState (Nmh (getPc (st p)) delS)
-                                      nextPc (updSt (state (st p)) delS))) m.
-
-  Variable initPc: Pc.
-  Variable initState: State.
-  Variable initRob: Rob.
-  Variable initPpc: Ppc.
+          (updP st p (Build_ProcState (Nmh (getPc (st p)) delS :: (hist (st p)))
+                                      nextPc (updSt (state (st p)) delS))) m
+  | Nothing: forall st m, CorrectSystem st m st m.
 
   Record SpecState :=
-    { hist': HistElem;
+    { hist': Hist;
       st: State;
       pc: Pc;
       p2m: Addr -> list Rq;
@@ -204,71 +202,82 @@ Section PerProc.
       ppc: Ppc
     }.
 
-  Section SpecFinal.
-    CoInductive SpecFinal: (Proc -> SpecState) -> Set :=
-    | Int:
-        forall state p h st pc p2m m2p wait rob ppc
-               h' st' pc' p2m' m2p' wait' rob' ppc',
-          state p = Build_SpecState h st pc p2m m2p wait rob ppc ->
-          Spec h st pc p2m m2p wait rob ppc
-               h' st' pc' p2m' m2p' wait' rob' ppc' Internal ->
-          SpecFinal (updP state p (Build_SpecState h' st' pc' p2m' m2p' wait' rob' ppc')) ->
-          SpecFinal state
-    | Ext:
-        forall state p h st pc p2m m2p wait rob ppc
-               h' st' pc' p2m' m2p' wait' rob' ppc' a x y,
-          state p = Build_SpecState h st pc p2m m2p wait rob ppc ->
-          Spec h st pc p2m m2p wait rob ppc
-               h' st' pc' p2m' m2p' wait' rob' ppc' External ->
-          p2m a = p2m' a ++ (x :: nil) ->
-          (forall a', a' <> a -> p2m a = p2m' a) ->
-          m2p' = m2p ++ (y :: nil) ->
-          SpecFinal (updP state p (Build_SpecState h' st' pc' p2m' m2p' wait' rob' ppc')) ->
-          SpecFinal state.
+  Inductive SpecFinal: (Proc -> SpecState) -> (Proc -> SpecState) -> Set :=
+  | Int:
+      forall state p h st pc p2m m2p wait rob ppc
+             h' st' pc' p2m' m2p' wait' rob' ppc',
+        state p = Build_SpecState h st pc p2m m2p wait rob ppc ->
+        Spec h st pc p2m m2p wait rob ppc
+             h' st' pc' p2m' m2p' wait' rob' ppc' Internal ->
+        SpecFinal state
+                  (updP state p (Build_SpecState h' st' pc' p2m' m2p' wait' rob' ppc'))
+  | Ext:
+      forall state p h st pc p2m m2p wait rob ppc
+             h' st' pc' p2m' m2p' wait' rob' ppc' a x y,
+        state p = Build_SpecState h st pc p2m m2p wait rob ppc ->
+        Spec h st pc p2m m2p wait rob ppc
+             h' st' pc' p2m' m2p' wait' rob' ppc' External ->
+        p2m a = p2m' a ++ (x :: nil) ->
+        (forall a', a' <> a -> p2m a = p2m' a) ->
+        m2p' = m2p ++ (y :: nil) ->
+        SpecFinal state
+                  (updP state p (Build_SpecState h' st' pc' p2m' m2p' wait' rob' ppc')).
 
+  CoInductive SpecFinal': (Proc -> SpecState) -> Set :=
+  | Build_SF: forall st1 st2, SpecFinal st1 st2 -> SpecFinal' st2 -> SpecFinal' st1.
+
+  Section SpecFinal.
     Definition incIs is a p a' p' :=
       match decAddr a a', decProc p p' with
         | left _, left _ => S (is a' p')
         | _, _ => is a' p'
       end.
 
-    CoFixpoint getRp spa (spf: SpecFinal spa) (is: Addr -> Proc -> Index) :=
-      match spf with
-        | Ext _ p _ _ _ _ _ _ _ _ _ _ _ _ _ _ _ _ a x y _ _ p2m1 _ m2prel future =>
-          match y with
-            | LoadRp _ v => Cons (Some (a, p, is a p, v)) (getRp future (incIs is a p))
-            | LoadCommitRp v => Cons (Some (a, p, is a p, v)) (getRp future (incIs is a p))
-            | StRp => Cons (Some (a, p, is a p, initData zero)) (getRp future (incIs is a p))
+    CoFixpoint getRp spa (spf': SpecFinal' spa) (is: Addr -> Proc -> Index) :=
+      match spf' with
+        | Build_SF _ _ spf future =>
+          match spf with
+            | Ext _ p _ _ _ _ _ _ _ _ _ _ _ _ _ _ _ _ a x y _ _ p2m1 _ m2prel =>
+              match y with
+                | LoadRp _ v => Cons (Some (a, p, is a p, v)) (getRp future (incIs is a p))
+                | LoadCommitRp v => Cons (Some (a, p, is a p, v))
+                                         (getRp future (incIs is a p))
+                | StRp => Cons (Some (a, p, is a p, initData zero))
+                               (getRp future (incIs is a p))
+              end
+            | Int _ _ _ _ _ _ _ _ _ _ _ _ _ _ _ _ _ _ _ _ =>
+              Cons None (getRp future is)
           end
-        | Int _ _ _ _ _ _ _ _ _ _ _ _ _ _ _ _ _ _ _ _ future =>
-          Cons None (getRp future is)
       end.
 
-    CoFixpoint getRq sta (spf: SpecFinal sta) :=
-      match spf with
-        | Ext _ p _ _ _ _ _ _ _ _ _ _ _ _ _ _ _ _ a x y _ _ p2m1 _ m2prel future =>
-          match x with
-            | LoadRq _ =>
-              fun a' p' =>
-                match decAddr a a', decProc p p' with
-                  | left _, left _ => Cons (Some (Ld, initData zero)) (getRq spf a' p')
-                  | _ , _ => Cons None (getRq spf a' p')
-                end
-            | LoadCommitRq =>
-              fun a' p' =>
-                match decAddr a a', decProc p p' with
-                  | left _, left _ => Cons (Some (Ld, initData zero)) (getRq spf a' p')
-                  | _ , _ => Cons None (getRq spf a' p')
-                end
-            | StoreRq v =>
-              fun a' p' =>
-                match decAddr a a', decProc p p' with
-                  | left _, left _ => Cons (Some (St, v)) (getRq spf a' p')
-                  | _ , _ => Cons None (getRq spf a' p')
-                end
+    CoFixpoint getRq sta (spf': SpecFinal' sta) :=
+      match spf' with
+        | Build_SF _ _ spf future =>
+          match spf with
+            | Ext _ p _ _ _ _ _ _ _ _ _ _ _ _ _ _ _ _ a x y _ _ p2m1 _ m2prel =>
+              match x with
+                | LoadRq _ =>
+                  fun a' p' =>
+                    match decAddr a a', decProc p p' with
+                      | left _, left _ => Cons (Some (Ld, initData zero)) (getRq future a' p')
+                      | _ , _ => Cons None (getRq future a' p')
+                    end
+                | LoadCommitRq =>
+                  fun a' p' =>
+                    match decAddr a a', decProc p p' with
+                      | left _, left _ => Cons (Some (Ld, initData zero)) (getRq future a' p')
+                      | _ , _ => Cons None (getRq future a' p')
+                    end
+                | StoreRq v =>
+                  fun a' p' =>
+                    match decAddr a a', decProc p p' with
+                      | left _, left _ => Cons (Some (St, v)) (getRq future a' p')
+                      | _ , _ => Cons None (getRq future a' p')
+                    end
+              end
+            | Int _ _ _ _ _ _ _ _ _ _ _ _ _ _ _ _ _ _ _ _ =>
+              fun a' p' => Cons None (getRq future a' p')
           end
-        | Int _ _ _ _ _ _ _ _ _ _ _ _ _ _ _ _ _ _ _ _ future =>
-          fun a' p' => Cons None (getRq future a' p')
       end.
 
     Fixpoint respFn' ls n :=
@@ -285,8 +294,17 @@ Section PerProc.
                  end
       end.
 
-    Variable spInit: Proc -> SpecState.
-    Variable spf: SpecFinal spInit.
+    Variable initPc: Pc.
+    Variable initState: State.
+    Variable initRob: Rob.
+    Variable initPpc: Ppc.
+
+    Definition normInit := Build_ProcState nil initPc initState.
+
+    Definition spInit := Build_SpecState nil initState initPc (fun a => nil) nil false
+                                         initRob initPpc.
+
+    Variable spf: SpecFinal' (fun p => spInit).
 
     Definition respFn := respFn' (getRp spf (fun a p => 0)).
 
@@ -313,7 +331,23 @@ Section PerProc.
 
     Variable isStoreAtomic: StoreAtomicity reqFn respFn.
 
+    Inductive CorrectSystemExec: (Proc -> ProcState) -> Mem -> Prop :=
+    | CsExec: forall st1 st2 m1 m2, CorrectSystem st1 m1 st2 m2 -> CorrectSystemExec st1 m1 ->
+                              CorrectSystemExec st2 m2
+    | CsInit: CorrectSystemExec (fun p => normInit) initData.
+
+    Inductive SpecSystemExec: (Proc -> SpecState) -> Prop :=
+    | SpExec: forall st1 st2, SpecFinal st1 st2 -> SpecSystemExec st1 ->
+                              SpecSystemExec st2
+    | SpInit: SpecSystemExec (fun p => spInit).
+
     Theorem histMatch:
-      
+      forall ss, SpecSystemExec ss ->
+                 exists ps m, CorrectSystemExec ps m /\
+                              forall p, hist (ps p) = hist' (ss p).
+    Proof.
+      admit.
+    Qed.
+
   End SpecFinal.
 End PerProc.
